Finish proof of corrected form of wpc_BufTxn__CommitWait
In particular, we can only get the durable_own_mapsto at the next generation,
not the current one. Old version remains admitted under the name
wpc_BufTxn__CommitWait_BAD so as to not break the simple.v proofs.

src/program_proof/buftxn/sep_buftxn_invariant.v
@@ -115,29 +115,6 @@ Section goose_lang.
       "H●latest" ∷ async_ctx γ.(buftxn_async_name) 1 σs
   .
 
-  (* this is for the entire txn manager, and relates it to some ghost state *)
-  Definition is_txn_system γ : iProp Σ :=
-    "Htxn_inv" ∷ ncinv N (txn_system_inv γ) ∗
-    "His_txn" ∷ ncinv invN (is_txn_always γ.(buftxn_txn_names)).
-
-  Lemma init_txn_system {E} l_txn γUnified dinit σs :
-    is_txn l_txn γUnified dinit ∗ ghost_var γUnified.(txn_crashstates) (3/4) σs ={E}=∗
-    ∃ γ, ⌜γ.(buftxn_txn_names) = γUnified⌝ ∗
-         is_txn_system γ.
-  Proof.
-    iIntros "[#Htxn Hasync]".
-    iMod (async_ctx_init σs) as (γasync) "H●async".
-    set (γ:={|buftxn_txn_names := γUnified; buftxn_async_name := γasync; |}).
-    iExists γ.
-    iMod (ncinv_alloc N E (txn_system_inv γ) with "[-]") as "($&Hcfupd)".
-    { iNext.
-      iExists _; iFrame. }
-    iModIntro.
-    simpl.
-    iSplit; first by auto.
-    iNamed "Htxn"; iFrame "#".
-  Qed.
-
   (* modify_token is an obligation from the buftxn_proof, which is how the txn
   invariant keeps track of exclusive ownership over an address. This proof has a
   more sophisticated notion of owning an address coming from the logical setup
@@ -171,6 +148,74 @@ Section goose_lang.
 
   Global Instance durable_mapsto_own_discretizable γ a obj: Discretizable (durable_mapsto_own γ a obj).
   Proof. apply _. Qed.
+
+  Definition crash_point γ logm crash_txn : iProp Σ :=
+    (* TODO: wrap crash_txn in an agree, give out an exchanger ghost name for
+    it *)
+    async_ctx γ.(buftxn_async_name) 1 logm ∗
+    ⌜(length (possible logm) = crash_txn + 1)%nat⌝.
+
+  Definition txn_durable_exchanger γ txn_id :=
+    heapspec.heapspec_durable_exchanger γ.(buftxn_txn_names).(txn_walnames) txn_id.
+
+  Lemma txn_durable_exchanger_use γ n lb :
+    txn_durable_exchanger γ n -∗
+    txn_durable γ lb -∗
+    ⌜ (lb ≤ n)%nat ⌝.
+  Proof. iIntros. iApply (heapspec.heapspec_durable_exchanger_use with "[$] [$]"). Qed.
+
+  Definition token_exchanger (a:addr) crash_txn γ γ' : iProp Σ :=
+    (∃ i, async.own_last_frag γ.(buftxn_async_name) a i) ∨
+    (async.own_last_frag γ'.(buftxn_async_name) a crash_txn ∗ modify_token γ' a).
+
+  Definition ephemeral_txn_val_exchanger (a:addr) crash_txn γ γ' : iProp Σ :=
+    ∃ v, ephemeral_txn_val γ.(buftxn_async_name) crash_txn a v ∗
+         ephemeral_txn_val γ'.(buftxn_async_name) crash_txn a v.
+
+  Definition addr_exchangers {A} txn γ γ' (m : gmap addr A) : iProp Σ :=
+    ([∗ map] a↦_ ∈ m,
+        token_exchanger a txn γ γ' ∗
+        ephemeral_txn_val_exchanger a txn γ γ')%I.
+
+  Definition sep_txn_exchanger γ γ' : iProp Σ :=
+    ∃ logm crash_txn,
+       "Hcrash_point" ∷ crash_point γ logm crash_txn ∗
+       "Hdurable_exchanger" ∷ txn_durable_exchanger γ crash_txn ∗
+       "#Hcrash_txn_durable" ∷ txn_durable γ' crash_txn ∗
+       "Hexchanger" ∷ addr_exchangers crash_txn γ γ' (latest logm)
+  .
+
+  Definition txn_cinv γ γ' : iProp Σ :=
+    □ |C={⊤}_0=> inv (N.@"txn") (sep_txn_exchanger γ γ').
+
+  (* this is for the entire txn manager, and relates it to some ghost state *)
+
+  Definition is_txn_system γ : iProp Σ :=
+    "Htxn_inv" ∷ ncinv N (txn_system_inv γ) ∗
+    "His_txn" ∷ ncinv invN (is_txn_always γ.(buftxn_txn_names)).
+
+  Definition is_txn_system_full γ γ' : iProp Σ :=
+    "His_txn_system" ∷ is_txn_system γ ∗
+    "Htxn_cinv" ∷ txn_cinv γ γ'.
+
+  Lemma init_txn_system {E} l_txn γUnified dinit σs :
+    is_txn l_txn γUnified dinit ∗ ghost_var γUnified.(txn_crashstates) (3/4) σs ={E}=∗
+    ∃ γ, ⌜γ.(buftxn_txn_names) = γUnified⌝ ∗
+         is_txn_system γ.
+  Proof.
+    iIntros "[#Htxn Hasync]".
+    iMod (async_ctx_init σs) as (γasync) "H●async".
+    set (γ:={|buftxn_txn_names := γUnified; buftxn_async_name := γasync; |}).
+    iExists γ.
+    iMod (ncinv_alloc N E (txn_system_inv γ) with "[-]") as "($&Hcfupd)".
+    { iNext.
+      iExists _; iFrame. }
+    iModIntro.
+    simpl.
+    iSplit; first by auto.
+    iNamed "Htxn"; iFrame "#".
+  Qed.
+
 
   Definition is_buftxn_mem l γ dinit γtxn γdurable : iProp Σ :=
     ∃ (mT: gmap addr versioned_object) anydirty,
@@ -468,6 +513,162 @@ Section goose_lang.
     - iApply (is_buftxn_wand with "Hctx").
       iIntros (mapsto) "!> [Hm $]".
       iApply "HP"; auto.
+  Qed.
+
+  Lemma exchange_big_sepM_addrs γ γ' (m0 m1 : gmap addr object) crash_txn :
+    dom (gset _) m0 ⊆ dom (gset _) m1 →
+    txn_durable γ' crash_txn -∗
+    addr_exchangers crash_txn γ γ' m1 -∗
+    ([∗ map] k0↦x ∈ m0, ephemeral_txn_val γ.(buftxn_async_name) crash_txn k0 x ∗
+                        (∃ i v, ephemeral_val_from γ.(buftxn_async_name) i k0 v)) -∗
+    addr_exchangers crash_txn γ γ' m1 ∗
+    [∗ map] k0↦x ∈ m0, durable_mapsto_own γ' k0 x.
+  Proof.
+    iIntros (Hdom) "#Hdur H1 H2".
+    rewrite /addr_exchangers.
+    iCombine "Hdur H1" as "H1".
+    iDestruct (big_sepM_mono_with_inv with "H1 H2") as "((_&$)&H)"; last iApply "H".
+    iIntros (k o Hlookup) "((#Hdur&Hm)&Hephem)".
+    assert (is_Some (m1 !! k)) as (v&?).
+    { apply elem_of_dom, Hdom, elem_of_dom. eauto. }
+    iDestruct (big_sepM_lookup_acc with "Hm") as "(H&Hm)"; first eassumption.
+    iDestruct "Hephem" as "(#Hval0&Hephem)".
+    iDestruct "Hephem" as (??) "(_&Htok0)".
+    iDestruct "H" as "(Htok&#Hval)".
+    iDestruct "Hval" as (?) "(Hval1&Hval2)".
+    iDestruct (ephemeral_txn_val_agree with "Hval0 Hval1") as %Heq. subst.
+    iDestruct "Htok" as "[Hl|(Hr1&Hr2)]".
+    { iExFalso. iDestruct "Hl" as (?) "H".
+      iApply (own_last_frag_conflict with "[$] [$]"). }
+    iSpecialize ("Hm" with "[Htok0]").
+    { iSplitL "Htok0".
+      - iLeft. eauto.
+      - iExists _. iFrame "#". }
+    iFrame "# ∗". iExists _. iFrame "# ∗".
+  Qed.
+
+  Lemma exchange_durable_mapsto γ γ' m k :
+    ("#Htxn_cinv" ∷ txn_cinv γ γ' ∗
+     "Hm" ∷ [∗ map] a↦v ∈ m, durable_mapsto γ a v) -∗
+    |C={⊤}_S k => ([∗ map] a↦v ∈ m, durable_mapsto_own γ' a v).
+  Proof.
+    iNamed 1.
+    iMod ("Htxn_cinv") as "#Hinv"; first lia.
+    iIntros "HC".
+    iInv ("Hinv") as ">H" "Hclo".
+    iNamed "H".
+    iDestruct "Hcrash_point" as "(Hasync&%Heq)".
+    iAssert (⌜dom (gset addr) m ⊆ dom (gset addr) logm.(latest)⌝)%I with "[Hm Hasync]" as "%Hdom2".
+    {
+      iInduction m as [| i x m] "IH" using map_ind.
+      { iPureIntro; set_solver. }
+      rewrite big_sepM_insert //.
+      iDestruct "Hm" as "(Hval1&Hval)".
+      iDestruct ("IH" with "[$] [$]") as %Hdom.
+      iDestruct "Hval1" as (?) "((?&?)&?)".
+      iDestruct (ephemeral_val_from_agree_latest with "[$] [$]") as %Hlookup.
+      iPureIntro. rewrite dom_insert.
+      assert (i ∈ dom (gset addr) (logm.(latest))).
+      { apply elem_of_dom. eauto. }
+      set_solver.
+    }
+
+    iAssert ((txn_durable_exchanger γ crash_txn ∗ async_ctx γ.(buftxn_async_name) 1 logm) ∗
+              ([∗ map] k0↦x ∈ m, ephemeral_txn_val γ.(buftxn_async_name) crash_txn k0 x
+                  ∗ (∃ (i : nat) (v : object), ephemeral_val_from γ.(buftxn_async_name) i k0 v)))%I
+            with "[Hasync Hdurable_exchanger Hm]" as "[[Hdurable_exchanger Hasync] Hm]".
+    {
+      iCombine "Hdurable_exchanger Hasync" as "H".
+      iDestruct (big_sepM_mono_with_inv with "H Hm") as "($&H)"; last iApply "H".
+      iIntros (? ? Hlookup) "((Hdurable_exchanger&Hasync)&Hm)".
+      iDestruct "Hm" as (?) "(?&?)".
+      iDestruct (txn_durable_exchanger_use with "[$] [$]") as %Hlb.
+      iDestruct (ephemeral_val_from_val with "Hasync [$]") as "#$".
+      { lia. }
+      { lia. }
+      iFrame. iExists _, _; eauto.
+    }
+    iDestruct (exchange_big_sepM_addrs with "[$] [$] Hm") as "(Hexchanger&Hval)".
+    { eauto. }
+    iMod ("Hclo" with "[Hexchanger Hdurable_exchanger Hasync]").
+    { iNext. iExists _, _. iFrame "# ∗". eauto. }
+    iModIntro. eauto.
+  Qed.
+
+  Lemma exchange_mapsto_commit γ γ' m0 m txn_id k :
+    dom (gset _) m0 ⊆ dom (gset _) m →
+    ("#Htxn_cinv" ∷ txn_cinv γ γ' ∗
+    "Hold_vals" ∷ ([∗ map] k↦x ∈ m0,
+          ∃ i : nat, txn_durable γ i ∗
+                     ephemeral_txn_val_range γ.(buftxn_async_name) i txn_id k x) ∗
+    "Hval" ∷ [∗ map] k↦x ∈ m, ephemeral_val_from γ.(buftxn_async_name) txn_id k x) -∗
+    |C={⊤}_S k => ([∗ map] a↦v ∈ m0, durable_mapsto_own γ' a v) ∨
+                  ([∗ map] a↦v ∈ m, durable_mapsto_own γ' a v).
+  Proof.
+    iIntros (Hdom1) "H". iNamed "H".
+    iMod ("Htxn_cinv") as "#Hinv"; first lia.
+    iIntros "HC".
+    iInv ("Hinv") as ">H" "Hclo".
+    iNamed "H".
+    iDestruct "Hcrash_point" as "(Hasync&%Heq)".
+    iAssert (⌜dom (gset addr) m ⊆ dom (gset addr) logm.(latest)⌝)%I with "[Hval Hasync]" as "%Hdom2".
+    {
+      clear Hdom1.
+      iInduction m as [| i x m] "IH" using map_ind.
+      { iPureIntro; set_solver. }
+      rewrite big_sepM_insert //.
+      iDestruct "Hval" as "(Hval1&Hval)".
+      iDestruct ("IH" with "[$] [$]") as %Hdom.
+      iDestruct (ephemeral_val_from_agree_latest with "[$] [$]") as %Hlookup.
+      iPureIntro. rewrite dom_insert.
+      assert (i ∈ dom (gset addr) (logm.(latest))).
+      { apply elem_of_dom. eauto. }
+      set_solver.
+    }
+
+    destruct (decide (crash_txn < txn_id)).
+    - (* We roll back, txn_id is not durable *)
+      iAssert (txn_durable_exchanger γ crash_txn ∗
+               ([∗ map] k0↦x ∈ m0, ephemeral_txn_val γ.(buftxn_async_name) crash_txn k0 x))%I
+        with "[Hold_vals Hdurable_exchanger]" as "(Hdurable_exchanger&#Hold)".
+      {
+        iDestruct (big_sepM_mono_with_inv with "Hdurable_exchanger Hold_vals") as "($&H)"; last iApply "H".
+        iIntros (?? Hlookup) "(Hdurable_exchanger&H)".
+        iDestruct "H" as (i) "(Hdurable&Hrange)".
+        iDestruct (txn_durable_exchanger_use with "[$] [$]") as %Hlb.
+        iFrame. iApply (ephemeral_txn_val_range_acc with "[$]").
+        lia.
+      }
+      iAssert ([∗ map] k0↦_ ∈ m, ∃ txn_id x, ephemeral_val_from γ.(buftxn_async_name) txn_id k0 x)%I
+       with "[Hval]" as "Hval".
+      { iApply (big_sepM_mono with "Hval"); eauto. }
+      iDestruct (big_sepM_dom with "Hval") as "Hval".
+      iDestruct (big_sepS_subseteq with "Hval") as "Hval"; eauto.
+      iDestruct (big_sepM_dom with "Hval") as "Hval".
+      iCombine "Hold Hval" as "Hval".
+      iEval (rewrite -big_sepM_sep) in "Hval".
+      iDestruct (exchange_big_sepM_addrs with "[$] [$] Hval") as "(Hexchanger&Hval)".
+      { etransitivity; last eassumption; eauto. }
+      iMod ("Hclo" with "[Hexchanger Hdurable_exchanger Hasync]").
+      { iNext. iExists _, _. iFrame "# ∗". eauto. }
+      iModIntro. eauto.
+    - (* We go forward, txn_id is durable *)
+      iAssert (async_ctx γ.(buftxn_async_name) 1 logm ∗
+                ([∗ map] k0↦x ∈ m, ephemeral_txn_val γ.(buftxn_async_name) crash_txn k0 x
+                    ∗ (∃ (i : nat) (v : object), ephemeral_val_from γ.(buftxn_async_name) i k0 v)))%I
+              with "[Hasync Hval]" as "[Hasync Hval]".
+      {iDestruct (big_sepM_mono_with_inv with "Hasync Hval") as "($&H)"; last iApply "H".
+       iIntros (? ? Hlookup) "(Hasync&Hval)".
+       iDestruct (ephemeral_val_from_val with "Hasync Hval") as "#$".
+       { lia. }
+       { lia. }
+       iFrame. iExists _, _; eauto.
+      }
+      iDestruct (exchange_big_sepM_addrs with "[$] [$] Hval") as "(Hexchanger&Hval)".
+      { eauto. }
+      iMod ("Hclo" with "[Hexchanger Hdurable_exchanger Hasync]").
+      { iNext. iExists _, _. iFrame "# ∗". eauto. }
+      iModIntro. eauto.
   Qed.
 
 End goose_lang.
